theories/Monad/Prenex.v
@@ -35,21 +35,20 @@ Import MonadNotations Pred Pred.Acc Pred.notations Pred.proofmode
 
 #[local] Set Implicit Arguments.
 
-Definition Prenex A := Option ◇⁺(List (Ṫy * Ṫy) * A).
-
 #[export] Instance pure_prenex : Pure Prenex :=
   fun A w a => Some (existT w (refl, (List.nil, a))).
 #[export] Instance bind_prenex : Bind Prefix Prenex :=
-  fun A B w (m : OptionDiamond Prefix (List (Ṫy * Ṫy) * A) w)
-      (f : Box Prefix (A ⇢ OptionDiamond Prefix (List (Ṫy * Ṫy) * B)) w) =>
+  fun A B w (m : Solved Prefix (List (Ṫy * Ṫy) * A) w)
+      (f : Box Prefix (A ⇢ Solved Prefix (List (Ṫy * Ṫy) * B)) w) =>
     '(C1,a1) <- m ;;
     '(C2,b2) <- f _ _ a1 ;;
     pure (persist C1 _ ++ C2, b2).
+#[export] Instance fail_prenex : Fail Prenex :=
+  fun A w => None.
 #[export] Instance tcm_prenex : TypeCheckM Prenex :=
   {| assert w τ1 τ2 := Some (existT w (refl, ([(τ1,τ2)], tt)));
      pick w := let α := world.fresh w in
                Some (existT (w ▻ α) (step, (List.nil, ṫy.var world.in_zero)));
-     fail A w := None;
   |}.
 
 #[local] Existing Instance instpred_prod_ty.
